Make make work.

solutions/sem_type_formers.v
@@ -7,112 +7,105 @@ formers, which given two semantic types [A] and [B], gives the semantic type of
 the product [A * B], i.e., values that are pairs where the first component
 belongs to [A] and the second component to [B]. *)
 
-Section types.
-  Context `{!heapG Σ}.
+(** * Base types *)
+(** Let us start with the simplest types of our language: unit, Boolean, and
+integers. The corresponding semantic types are defined as follows: *)
+Definition sem_ty_unit {Σ} : sem_ty Σ := SemTy (λ w,
+  ⌜ w = #() ⌝)%I.
+Definition sem_ty_bool {Σ} : sem_ty Σ := SemTy (λ w,
+  ∃ b : bool, ⌜ w = #b ⌝)%I.
+Definition sem_ty_int {Σ} : sem_ty Σ := SemTy (λ w,
+  ∃ n : Z, ⌜ w = #n ⌝)%I.
 
-  (** * Base types *)
-  (** Let us start with the simplest types of our language: unit and Boolean.
-  The corresponding semantic types are defined as follows: *)
-  Definition sem_ty_unit : sem_ty Σ := SemTy (λ w,
-    ⌜ w = #() ⌝)%I.
-  Definition sem_ty_bool : sem_ty Σ := SemTy (λ w,
-    ∃ b : bool, ⌜ w = #b ⌝)%I.
+(** These interpretations are exactly what you would expect: the only value
+of the unit type is the unit value [()], the values of the Boolean type are
+the elements of the Coq type [bool] (i.e. [true] and [false]), and the values
+of the integer type are the integer literals. *)
 
-  (** These interpretations are exactly what you would expect: the only value
-  of the unit type is the unit value [()], the values of the Boolean type are
-  the elements of the Coq type [bool] (i.e. [true] and [false]). *)
+(** * Products and sums *)
+(** The semantic type former for products is as follows: *)
+Definition sem_ty_prod {Σ} (A1 A2 : sem_ty Σ) : sem_ty Σ := SemTy (λ w,
+  ∃ w1 w2, ⌜w = (w1, w2)%V⌝ ∧ A1 w1 ∧ A2 w2)%I.
 
-  (** ** Exercise (sem_ty_int, easy) *)
-  (** Define the semantic version of the type of integers. *)
-  (* REMOVE *) Definition sem_ty_int : sem_ty Σ := SemTy (λ w,
-    ∃ n : Z, ⌜ w = #n ⌝)%I.
+(** Values of the product type over [A1] and [A2] should be tuples [(w1, w2)],
+where [w1] and [w2] should values in the semantic type [A1] and [A2],
+respectively. *)
 
-  (** * Products and sums *)
-  (** The semantic type former for products is as follows: *)
-  Definition sem_ty_prod (A1 A2 : sem_ty Σ) : sem_ty Σ := SemTy (λ w,
-    ∃ w1 w2, ⌜w = (w1, w2)%V⌝ ∧ A1 w1 ∧ A2 w2)%I.
+(** The type former for sums is similar. *)
+Definition sem_ty_sum {Σ} (A1 A2 : sem_ty Σ) : sem_ty Σ := SemTy (λ w,
+    (∃ w1, ⌜w = InjLV w1⌝ ∧ A1 w1)
+  ∨ (∃ w2, ⌜w = InjRV w2⌝ ∧ A2 w2))%I.
 
-  (** Values of the product type over [A1] and [A2] should be tuples [(w1, w2)],
-  where [w1] and [w2] should values in the semantic type [A1] and [A2],
-  respectively. *)
+(** * Functions *)
+(** The semantic type former for functions is as follows: *)
+Definition sem_ty_arr `{!heapG Σ} (A1 A2 : sem_ty Σ) : sem_ty Σ := SemTy (λ w,
+  □ ∀ v, A1 v -∗ WP App w v {{ A2 }})%I.
+(** This definition is very close to the usual way of defining the type
+former for the function type [A1 → A2] in traditional logical relations: it
+expresses that arguments of semantic type [A1] are mapped to results of
+semantic type [A2]. The definition makes two of two features of Iris:
 
-  (** ** Exercise (sem_ty_sum, moderate) *)
-  (** Define the semantic type former for sums. *)
-  (* REMOVE *) Definition sem_ty_sum (A1 A2 : sem_ty Σ) : sem_ty Σ := SemTy (λ w,
-      (∃ w1, ⌜w = InjLV w1⌝ ∧ A1 w1)
-    ∨ (∃ w2, ⌜w = InjRV w2⌝ ∧ A2 w2))%I.
+- The weakest precondition [WP e {{ Φ }}].
+- The persistence modality [□]. Recall that semantic types are persistent Iris
+  predicates. However, even if both [P] and [Q] are persistent propositions,
+  the magic wand [P -∗ Q] is not necessarily persistent. Hence, we use the [□
+  modality to make the magic wand persistent.
+*)
 
-  (** * Functions *)
-  (** The semantic type former for functions is as follows: *)
-  Definition sem_ty_arr (A1 A2 : sem_ty Σ) : sem_ty Σ := SemTy (λ w,
-    □ ∀ v, A1 v -∗ WP App w v {{ A2 }})%I.
-  (** This definition is very close to the usual way of defining the type
-  former for the function type [A1 → A2] in traditional logical relations: it
-  expresses that arguments of semantic type [A1] are mapped to results of
-  semantic type [A2]. The definition makes two of two features of Iris:
+(** * Polymorphism and existentials *)
+Definition sem_ty_forall `{!heapG Σ} (C : sem_ty Σ → sem_ty Σ) : sem_ty Σ := SemTy (λ w,
+  □ ∀ A : sem_ty Σ, WP w #() {{ w, C A w }})%I.
+Definition sem_ty_exist {Σ} (C : sem_ty Σ → sem_ty Σ) : sem_ty Σ := SemTy (λ w,
+  ∃ A : sem_ty Σ, C A w)%I.
+(** The interpretations of these types are fairly straightforward.
+Given a higher-order type former [C] that maps semantic types to
+semantic types, we define the universal type [sem_ty_forall A]
+using the universal quantification in Iris. That is, a value [w]
+is considered a polymorphic value if for any semantic type [A],
+when [w] is specialized to the type [A] (written as [w #()] as
+(semantic) types never appear in terms in our untyped syntax)
+the _resulting expression_ is an expression in the semantics of
+the type [C A] (defined using WP).
 
-  - The weakest precondition [WP e {{ Φ }}].
-  - The persistence modality [□]. Recall that semantic types are persistent Iris
-    predicates. However, even if both [P] and [Q] are persistent propositions,
-    the magic wand [P -∗ Q] is not necessarily persistent. Hence, we use the [□
-    modality to make the magic wand persistent.
-  *)
+Similarly, given a higher-order type former [C] that maps
+semantic types to semantic types, we define the existential type
+[sem_ty_exist A] using the existential quantification in Iris.
 
-  (** * Polymorphism and existentials *)
-  Definition sem_ty_forall (C : sem_ty Σ → sem_ty Σ) : sem_ty Σ := SemTy (λ w,
-    □ ∀ A : sem_ty Σ, WP w #() {{ w, C A w }})%I.
-  Definition sem_ty_exist (C : sem_ty Σ → sem_ty Σ) : sem_ty Σ := SemTy (λ w,
-    ∃ A : sem_ty Σ, C A w)%I.
-  (** The interpretations of these types are fairly straightforward.
-  Given a higher-order type former [C] that maps semantic types to
-  semantic types, we define the universal type [sem_ty_forall A]
-  using the universal quantification in Iris. That is, a value [w]
-  is considered a polymorphic value if for any semantic type [A],
-  when [w] is specialized to the type [A] (written as [w #()] as
-  (semantic) types never appear in terms in our untyped syntax)
-  the _resulting expression_ is an expression in the semantics of
-  the type [C A] (defined using WP).
+Notice how the impredicative nature of Iris propositions and
+predicates allows us to quantify over Iris predicates to define
+an Iris predicate. This is crucial for giving semantics to
+parametric polymorphism, i.e., universal and existential types.
 
-  Similarly, given a higher-order type former [C] that maps
-  semantic types to semantic types, we define the existential type
-  [sem_ty_exist A] using the existential quantification in Iris.
+Remark: notice that for technical reasons (related to the value
+restriction problem in ML-like languages) universally quantified
+expressions are not evaluated until they are applied to a
+specific type. *)
 
-  Notice how the impredicative nature of Iris propositions and
-  predicates allows us to quantify over Iris predicates to define
-  an Iris predicate. This is crucial for giving semantics to
-  parametric polymorphism, i.e., universal and existential types.
+(** * References *)
+Definition tyN := nroot .@ "ty".
+Definition sem_ty_ref `{!heapG Σ} (A : sem_ty Σ) : sem_ty Σ := SemTy (λ w,
+  ∃ l : loc, ⌜w = #l⌝ ∧ inv (tyN .@ l) (∃ v, l ↦ v ∗ A v))%I.
+(** Intuitively, values of the reference type [sem_ty_ref A] should
+be locations [l] that hold a value [w] in the semantic type [A] at
+all times. In order to express this intuition in a formal way, we
+make use of two features of Iris:
 
-  Remark: notice that for technical reasons (related to the value
-  restriction problem in ML-like languages) universally quantified
-  expressions are not evaluated until they are applied to a
-  specific type. *)
+- The points-to connective l ↦ v (from vanilla separation logic)
+  provides exclusive ownership of the location l with value
+  v. The points-to connective is an ephemeral proposition, and
+  necessarily not a persistent proposition.
 
-  (** * References *)
-  Definition tyN := nroot .@ "ty".
-  Definition sem_ty_ref (A : sem_ty Σ) : sem_ty Σ := SemTy (λ w,
-    ∃ l : loc, ⌜w = #l⌝ ∧ inv (tyN .@ l) (∃ v, l ↦ v ∗ A v))%I.
-  (** Intuitively, values of the reference type [sem_ty_ref A] should
-  be locations [l] that hold a value [w] in the semantic type [A] at
-  all times. In order to express this intuition in a formal way, we
-  make use of two features of Iris:
+- The invariant assertion [inv N P] expresses that a (typically
+  ephemeral) proposition [P] holds at all times -- i.e., [P] is
+  invariant. The invariant assertion is persistent.
+*)
 
-  - The points-to connective l ↦ v (from vanilla separation logic)
-    provides exclusive ownership of the location l with value
-    v. The points-to connective is an ephemeral proposition, and
-    necessarily not a persistent proposition.
-
-  - The invariant assertion [inv N P] expresses that a (typically
-    ephemeral) proposition [P] holds at all times -- i.e., [P] is
-    invariant. The invariant assertion is persistent.
-  *)
-
-  (** Remark: Iris is also capable giving semantics to recursive
-  types. However, for the sake of simplicity we did not consider
-  recursive types for this tutorial. In particular, to give the
-  semantics of recursive types one needs to use Iris's guarded
-  fixpoints, which require some additional bookkeeping related to
-  contractiveness. *)
-End types.
+(** Remark: Iris is also capable giving semantics to recursive
+types. However, for the sake of simplicity we did not consider
+recursive types for this tutorial. In particular, to give the
+semantics of recursive types one needs to use Iris's guarded
+fixpoints, which require some additional bookkeeping related to
+contractiveness. *)
 
 (** We introduce nicely looking notations for our semantic types. This allows
 us to write lemmas, for example, the compatibility lemmas, in a readable way. *)
@@ -129,10 +122,10 @@ Notation "'ref' A" := (sem_ty_ref A) : sem_ty_scope.
 (** A [Params t n] instance tells Coq's setoid rewriting mechanism *not* to
 rewrite in the first [n] arguments of [t]. These instances tend to make the
 setoid rewriting mechanism a lot faster. This code is mostly boilerplate. *)
-Instance: Params (@sem_ty_arr) 1 := {}.
 Instance: Params (@sem_ty_prod) 1 := {}.
 Instance: Params (@sem_ty_sum) 1 := {}.
-Instance: Params (@sem_ty_forall) 1 := {}.
+Instance: Params (@sem_ty_arr) 1 := {}.
+Instance: Params (@sem_ty_forall) 2 := {}.
 Instance: Params (@sem_ty_exist) 1 := {}.
 Instance: Params (@sem_ty_ref) 2 := {}.
 
