exercises/compatibility.v
@@ -58,29 +58,21 @@ Section compatibility.
     iDestruct 1 as (w1 w2 ->) "[??]". by wp_pures.
   Qed.
   Lemma Snd_sem_typed Γ e A1 A2 : Γ ⊨ e : A1 * A2 -∗ Γ ⊨ Snd e : A2.
-  Proof.
-    iIntros "#H" (vs) "!# #HΓ /=".
-    wp_apply (wp_wand with "(H [//])"); iIntros (w).
-    iDestruct 1 as (w1 w2 ->) "[??]". by wp_pures.
-  Qed.
+  Proof. (* FILL IN YOUR PROOF *) Admitted.
 
   Lemma InjL_sem_typed Γ e A1 A2 : Γ ⊨ e : A1 -∗ Γ ⊨ InjL e : A1 + A2.
-  Proof. (* FILL IN YOUR PROOF *) Qed.
-  (* REMOVE *) Lemma InjR_sem_typed Γ e A1 A2 : Γ ⊨ e : A2 -∗ Γ ⊨ InjR e : A1 + A2.
-  Proof.
-    iIntros "#H" (vs) "!# #HΓ /=".
-    wp_apply (wp_wand with "(H [//])"); iIntros (w) "#HA".
-    wp_pures. iRight. iExists w. auto.
-  Qed.
+  Proof. (* FILL IN YOUR PROOF *) Admitted.
+  Lemma InjR_sem_typed Γ e A1 A2 : Γ ⊨ e : A2 -∗ Γ ⊨ InjR e : A1 + A2.
+  Proof. (* FILL IN YOUR PROOF *) Admitted.
   Lemma Case_sem_typed Γ e e1 e2 A1 A2 B :
     Γ ⊨ e : A1 + A2 -∗ Γ ⊨ e1 : (A1 → B) -∗ Γ ⊨ e2 : (A2 → B) -∗
     Γ ⊨ Case e e1 e2 : B.
-  Proof. (* FILL IN YOUR PROOF *) Qed.
+  Proof. (* FILL IN YOUR PROOF *) Admitted.
 
   (** * Functions *)
   Lemma Rec_sem_typed Γ f x e A1 A2 :
     binder_insert f (A1 → A2)%sem_ty (binder_insert x A1 Γ) ⊨ e : A2 -∗
-    Γ ⊨ (rec: f x. (* FILL IN HERE *) Admitted.
+    Γ ⊨ (rec: f x := e) : (A1 → A2).
   Proof.
     iIntros "#H" (vs) "!# #HΓ /=". wp_pures. iLöb as "IH".
     iIntros "!#" (v) "#HA1". wp_pures. set (r := RecV f x _).
@@ -109,11 +101,11 @@ Section compatibility.
   Qed.
 
   Lemma Pack_sem_typed Γ e C A : Γ ⊨ e : C A -∗ Γ ⊨ (pack: e) : ∃ A, C A.
-  Proof. (* FILL IN YOUR PROOF *) Qed.
+  Proof. (* FILL IN YOUR PROOF *) Admitted.
   Lemma Unpack_sem_typed Γ x e1 e2 C B :
     (Γ ⊨ e1 : ∃ A, C A) -∗ (∀ A, binder_insert x (C A) Γ ⊨ e2 : B) -∗
     Γ ⊨ (unpack: x := e1 in e2) : B.
-  Proof. (* FILL IN YOUR PROOF *) Qed.
+  Proof. (* FILL IN YOUR PROOF *) Admitted.
 
   (** ** Heap operations *)
   Lemma Alloc_sem_typed Γ e A : Γ ⊨ e : A -∗ Γ ⊨ ref e : ref A.
@@ -134,15 +126,15 @@ Section compatibility.
   Qed.
   Lemma Store_sem_typed Γ e1 e2 A :
     Γ ⊨ e1 : ref A -∗ Γ ⊨ e2 : A -∗ Γ ⊨ (e1 <- e2) : ().
-  Proof. (* FILL IN YOUR PROOF *) Qed.
+  Proof. (* FILL IN YOUR PROOF *) Admitted.
   Lemma FAA_sem_typed Γ e1 e2 :
     Γ ⊨ e1 : ref sem_ty_int -∗ Γ ⊨ e2 : sem_ty_int -∗ Γ ⊨ FAA e1 e2 : sem_ty_int.
-  Proof. (* FILL IN YOUR PROOF *) Qed.
+  Proof. (* FILL IN YOUR PROOF *) Admitted.
   Lemma CmpXchg_sem_typed Γ A e1 e2 e3 :
     SemTyUnboxed A →
     Γ ⊨ e1 : ref A -∗ Γ ⊨ e2 : A -∗ Γ ⊨ e3 : A -∗
     Γ ⊨ CmpXchg e1 e2 e3 : A * sem_ty_bool.
-  Proof. (* FILL IN YOUR PROOF *) Qed.
+  Proof. (* FILL IN YOUR PROOF *) Admitted.
 
   (** ** Operators *)
   Lemma UnOp_sem_typed Γ e op A B :
@@ -154,16 +146,16 @@ Section compatibility.
   Qed.
   Lemma BinOp_sem_typed Γ e1 e2 op A1 A2 B :
     SemTyBinOp op A1 A2 B → Γ ⊨ e1 : A1 -∗ Γ ⊨ e2 : A2 -∗ Γ ⊨ BinOp op e1 e2 : B.
-  Proof. (* FILL IN YOUR PROOF *) Qed.
+  Proof. (* FILL IN YOUR PROOF *) Admitted.
 
   Lemma If_sem_typed Γ e e1 e2 B :
     Γ ⊨ e : sem_ty_bool -∗ Γ ⊨ e1 : B -∗ Γ ⊨ e2 : B -∗
     Γ ⊨ (if: e then e1 else e2) : B.
-  Proof. (* FILL IN YOUR PROOF *) Qed.
+  Proof. (* FILL IN YOUR PROOF *) Admitted.
 
   (** ** Fork *)
   Lemma Fork_sem_typed Γ e : Γ ⊨ e : () -∗ Γ ⊨ Fork e : ().
-  Proof. (* FILL IN YOUR PROOF *) Qed.
+  Proof. (* FILL IN YOUR PROOF *) Admitted.
 
   (** * Compatibility rules for value typing *)
   (** ** Base types *)
@@ -172,7 +164,7 @@ Section compatibility.
   Lemma BoolV_sem_typed (b : bool) : (⊨ᵥ #b : sem_ty_bool)%I.
   Proof. by iExists b. Qed.
   Lemma IntV_sem_typed (n : Z) : (⊨ᵥ #n : sem_ty_int)%I.
-  Proof. (* FILL IN YOUR PROOF *) Qed.
+  Proof. (* FILL IN YOUR PROOF *) Admitted.
 
   (** ** Products and sums *)
   Lemma PairV_sem_typed v1 v2 τ1 τ2 :
