exercises/language.v
@@ -233,7 +233,7 @@ You should prove this lemma.
 
 Hint: [wp_pures] also executes the [+] operator. Carefully check how it affects
 the embedded [#] and convince yourself why that makes sense. *)
-Proof. (* FILL IN YOUR PROOF *) Qed.
+Proof. (* FILL IN YOUR PROOF *) Admitted.
 
 (** ** Reasoning about higher-order functions *)
 (** For the next example, let us consider the higher-order function [twice].
@@ -336,7 +336,7 @@ Lemma wp_add_two_ref `{!heapG Σ} l (x : Z) :
 about addition on [Z] (or the [replace] or [rewrite (_ : x = y)] tactic with
 [lia]) to turn [2 + x] into [1 + (1 + x)]. Tactics like [replace] and [rewrite]
 work operate both on the MoSeL proof goal and the MoSeL proof context. *)
-Proof. (* FILL IN YOUR PROOF *) Qed.
+Proof. (* FILL IN YOUR PROOF *) Admitted.
 
 (** ** Reasoning about higher-order state *)
 (** To see how Iris can be used to reason about higher-order state---that is,
@@ -407,7 +407,7 @@ Definition add_two_fancy : val := λ: "x",
 
 Lemma wp_add_two_fancy `{!heapG Σ} (x : Z) :
   WP add_two_fancy #x {{ w, ⌜ w = #(2 + x) ⌝ }}%I.
-Proof. (* FILL IN YOUR PROOF *) Qed.
+Proof. (* FILL IN YOUR PROOF *) Admitted.
 
 (** * Reasoning about "unsafe" programs *)
 (** Since HeapLang is an untyped language, we can write down arbitrary
@@ -438,4 +438,4 @@ Definition unsafe_ref : val := λ: <>,
 
 Lemma wp_unsafe_ref `{!heapG Σ} :
   WP unsafe_ref #() {{ v, ⌜ v = #true ⌝ }}%I.
-Proof. (* FILL IN YOUR PROOF *) Qed.
+Proof. (* FILL IN YOUR PROOF *) Admitted.
