exercises/parametricity.v
@@ -27,20 +27,20 @@ Section parametricity.
     (∀ `{!heapG Σ}, (∅ ⊨ e : ∀ A, A)%I) →
     rtc erased_step ([e <_>]%E, σ) (of_val w :: es, σ') →
     False.
-  Proof. (* FILL IN YOUR PROOF *) Qed.
+  Proof. (* FILL IN YOUR PROOF *) Admitted.
 
   (** * Exercise (boolean_param, moderate) *)
   Lemma boolean_param `{!heapPreG Σ} e (v1 v2 : val) σ w es σ' :
     (∀ `{!heapG Σ}, (∅ ⊨ e : ∀ A, A → A → A)%I) →
     rtc erased_step ([e <_> v1 v2]%E, σ) (of_val w :: es, σ') → w = v1 ∨ w = v2.
-  Proof. (* FILL IN YOUR PROOF *) Qed.
+  Proof. (* FILL IN YOUR PROOF *) Admitted.
 
   (** * Exercise (nat_param, hard) *)
   Lemma nat_param `{!heapPreG Σ} e σ w es σ' :
     (∀ `{!heapG Σ}, (∅ ⊨ e : ∀ A, (A → A) → A → A)%I) →
     rtc erased_step ([e <_> (λ: "n", "n" + #1)%V #0]%E, σ)
       (of_val w :: es, σ') → ∃ n : nat, w = #n.
-  Proof. (* FILL IN YOUR PROOF *) Qed.
+  Proof. (* FILL IN YOUR PROOF *) Admitted.
 
   (** * Exercise (strong_nat_param, hard) *)
   Lemma strong_nat_param `{!heapPreG Σ} e σ w es σ' (vf vz : val) φ :
@@ -50,5 +50,5 @@ Section parametricity.
       (Φ vz)%I ∧
       (∀ w, Φ w -∗ ⌜φ w⌝)%I) →
     rtc erased_step ([e <_> vf vz]%E, σ) (of_val w :: es, σ') → φ w.
-  Proof. (* FILL IN YOUR PROOF *) Qed.
+  Proof. (* FILL IN YOUR PROOF *) Admitted.
 End parametricity.
