exercises/polymorphism.v
@@ -44,4 +44,4 @@ Lemma wp_swap_poly `{!heapG Σ} l1 l2 v1 v2 :
   l1 ↦ v1 -∗
   l2 ↦ v2 -∗
   WP swap_poly <_> #l1 #l2 {{ v, ⌜ v = #() ⌝ ∗ l1 ↦ v2 ∗ l2 ↦ v1 }}.
-Proof. (* FILL IN YOUR PROOF *) Qed.
+Proof. (* FILL IN YOUR PROOF *) Admitted.
